README.md
@@ -4,3 +4,5 @@ How to install Lurk:
 1. `git clone https://github.com/lurk-lab/lurk.git`
 2. `cd lurk`
 3. `cargo install --path . --locked`
+
+Lurk docs: https://docs.argument.xyz/
